\section*{Laws of Boolean Algebra}
\begin{tabularx}{\linewidth}{lXX}
	\toprule
	\textbf{Name}         & \textbf{AND}                                                  & \textbf{OR}                                                     \\
	\midrule
	Identity Law          & $x \cdot 1 = x$                                               & $x + 0 = x$                                                     \\
	Invert/Complement Law & $x \cdot x' = 0$                                              & $x + x' = 1$                                                    \\
	Commutative Law       & $x \cdot y = y \cdot x$                                       & $x + y = y + x$                                                 \\
	Associative Law       & $x \cdot (y \cdot z) = (x \cdot y) \cdot z$                   & $x + (y + z) = (x + y) + z$                                     \\
	Distributive Law      & $x \cdot (y + z) = x \cdot y + x \cdot z$                     & $x + y \cdot z = (x + y) \cdot (x + z)$                         \\
	\midrule
	Idempotency           & $x \cdot x = x$                                               & $x + x = x$                                                     \\
	Zero/One Element      & $x \cdot 0 = 0$                                               & $x + 1 = 1$                                                     \\
	Involution            & $(x')' = x$                                                   &                                                                 \\
	Absorption 1          & $x + x \cdot y = x$                                           & $x \cdot (x + y) = x$                                           \\
	Absorption 2          & $x + x' \cdot y = x + y$                                      & $x \cdot (x' + y) = x \cdot y$                                  \\
	DeMorgan's Law        & $(x \cdot y)' = x' + y'$                                      & $(x + y)' = x' \cdot y'$                                        \\
	Consensus             & $x \cdot y + x' \cdot z + y \cdot z = x \cdot y + x' \cdot z$ & $(x + y) \cdot (x' + z) \cdot (y + z) = (x + y) \cdot (x' + z)$ \\
	\bottomrule
\end{tabularx}
